more

Weidenbach_Book/IsaSAT.thy
@@ -59,19 +59,39 @@ definition IsaSAT :: \<open>nat clause_l list \<Rightarrow> nat literal list opt
     let \<A>\<^sub>i\<^sub>n' = mset_set (extract_atms_clss CS {});
     ASSERT(isasat_input_bounded \<A>\<^sub>i\<^sub>n');
     ASSERT(distinct_mset \<A>\<^sub>i\<^sub>n');
-    let S = isasat_input_ops.init_state_wl \<A>\<^sub>i\<^sub>n';
-    let S = to_init_state S;
-    T \<leftarrow> init_dt_wl CS S;
-    let T = from_init_state T;
-    if \<not>get_conflict_wl_is_None_init T
-    then RETURN (None)
-    else if CS = [] then RETURN (Some [])
+    b \<leftarrow> SPEC(\<lambda>_. True);
+    if b \<and> length CS < uint_max - 1
+    then do {
+      let S = isasat_input_ops.init_state_wl \<A>\<^sub>i\<^sub>n';
+      let S = to_init_state S;
+      T \<leftarrow> init_dt_wl CS S;
+      let T = from_init_state T;
+      if \<not>get_conflict_wl_is_None_init T
+      then RETURN (None)
+      else if CS = [] then RETURN (Some [])
+      else do {
+         ASSERT(\<A>\<^sub>i\<^sub>n' \<noteq> {#});
+         ASSERT(isasat_input_bounded_nempty \<A>\<^sub>i\<^sub>n');
+         let T = finalise_init T;
+         U \<leftarrow> isasat_input_ops.cdcl_twl_stgy_prog_break_wl_D \<A>\<^sub>i\<^sub>n' T;
+         RETURN (if get_conflict_wl U = None then extract_model_of_state U else extract_stats U)
+      }
+    }
     else do {
-       ASSERT(\<A>\<^sub>i\<^sub>n' \<noteq> {#});
-       ASSERT(isasat_input_bounded_nempty \<A>\<^sub>i\<^sub>n');
-       let T = finalise_init T;
-       U \<leftarrow> isasat_input_ops.cdcl_twl_stgy_prog_wl_D \<A>\<^sub>i\<^sub>n' T;
-       RETURN (if get_conflict_wl U = None then extract_model_of_state U else extract_stats U)
+      let S = isasat_input_ops.init_state_wl \<A>\<^sub>i\<^sub>n';
+      let S = to_init_state S;
+      T \<leftarrow> init_dt_wl CS S;
+      let T = from_init_state T;
+      if \<not>get_conflict_wl_is_None_init T
+      then RETURN (None)
+      else if CS = [] then RETURN (Some [])
+      else do {
+         ASSERT(\<A>\<^sub>i\<^sub>n' \<noteq> {#});
+         ASSERT(isasat_input_bounded_nempty \<A>\<^sub>i\<^sub>n');
+         let T = finalise_init T;
+         U \<leftarrow> isasat_input_ops.cdcl_twl_stgy_prog_wl_D \<A>\<^sub>i\<^sub>n' T;
+         RETURN (if get_conflict_wl U = None then extract_model_of_state U else extract_stats U)
+      }
     }
   }\<close>
 
@@ -142,17 +162,111 @@ lemma init_dt_wl_code_refine[sepref_fr_rules]:
             \<open>virtual_copy_assn \<A>\<^sub>i\<^sub>n (fst (fst a))\<close>])
   done
 
+lemma init_dt_wl_fast_code_refine[sepref_fr_rules]:
+  \<open>(uncurry2 (\<lambda>_. init_dt_wl_fast_code), uncurry2 (isasat_input_ops.init_dt_wl_heur_fast))
+  \<in> [\<lambda>((N, S), S'). isasat_input_bounded \<A>\<^sub>i\<^sub>n \<and> N = \<A>\<^sub>i\<^sub>n]\<^sub>a
+    virtual_copy_assn\<^sup>k *\<^sub>a (list_assn (list_assn unat_lit_assn))\<^sup>d *\<^sub>a
+     (isasat_input_ops.isasat_init_fast_assn \<A>\<^sub>i\<^sub>n)\<^sup>d \<rightarrow>
+    isasat_input_ops.isasat_init_fast_assn \<A>\<^sub>i\<^sub>n\<close>
+  unfolding PR_CONST_def
+  unfolding hfref_def hn_refine_def
+  apply (subst in_pair_collect_simp)
+  apply (intro allI impI)
+  subgoal for a c
+    using init_dt_wl_fast_code.refine[of \<A>\<^sub>i\<^sub>n,
+      unfolded in_pair_collect_simp hfref_def hn_refine_def PR_CONST_def,
+      rule_format, of \<open>(snd (fst c), snd c)\<close> \<open>(snd (fst a), snd a)\<close>]
+    by (cases a)
+       (sep_auto dest!: frame_rule_left[of \<open>_ * isasat_input_ops.isasat_init_fast_assn _ _ _\<close> _ _
+            \<open>virtual_copy_assn \<A>\<^sub>i\<^sub>n (fst (fst a))\<close>])
+  done
+
 definition (in -)convert_state where
   \<open>convert_state _ S = S\<close>
 
-lemma (in -) convert_state_hnr[sepref_fr_rules]:
+lemma (in -) convert_state_hnr:
   \<open>(uncurry (return oo (\<lambda>_ S. S)), uncurry (RETURN oo convert_state))
    \<in> [\<lambda>(N, S). N = \<A>\<^sub>i\<^sub>n \<and> N = \<A>\<^sub>i\<^sub>n']\<^sub>a
      virtual_copy_assn\<^sup>k *\<^sub>a (isasat_input_ops.isasat_init_assn \<A>\<^sub>i\<^sub>n)\<^sup>d \<rightarrow>
      isasat_input_ops.isasat_init_assn \<A>\<^sub>i\<^sub>n'\<close>
   by sepref_to_hoare (sep_auto simp: convert_state_def)
 
+
+lemma (in -) convert_state_fast_hnr:
+  \<open>(uncurry (return oo (\<lambda>_ S. S)), uncurry (RETURN oo convert_state))
+   \<in> [\<lambda>(N, S). N = \<A>\<^sub>i\<^sub>n \<and> N = \<A>\<^sub>i\<^sub>n']\<^sub>a
+     virtual_copy_assn\<^sup>k *\<^sub>a (isasat_input_ops.isasat_init_fast_assn \<A>\<^sub>i\<^sub>n)\<^sup>d \<rightarrow>
+     isasat_input_ops.isasat_init_fast_assn \<A>\<^sub>i\<^sub>n'\<close>
+  by sepref_to_hoare (sep_auto simp: convert_state_def)
+
+definition IsaSAT_use_fast_mode where
+  \<open>IsaSAT_use_fast_mode = True\<close>
+
+lemma IsaSAT_use_fast_mode[sepref_fr_rules]:
+  \<open>(uncurry0 (return IsaSAT_use_fast_mode), uncurry0 (RETURN IsaSAT_use_fast_mode)) 
+   \<in> unit_assn\<^sup>k \<rightarrow>\<^sub>a bool_assn\<close>
+  by sepref_to_hoare sep_auto
+
 definition IsaSAT_heur :: \<open>nat clause_l list \<Rightarrow> (nat literal list option \<times> stats) nres\<close> where
+  \<open>IsaSAT_heur CS = do{
+    ASSERT(\<forall>C\<in>set CS. \<forall>L\<in>set C. nat_of_lit L \<le> uint_max);
+    let \<A>\<^sub>i\<^sub>n' = mset_set (extract_atms_clss CS {});
+    ASSERT(isasat_input_bounded \<A>\<^sub>i\<^sub>n');
+    ASSERT(distinct_mset \<A>\<^sub>i\<^sub>n');
+    let \<A>\<^sub>i\<^sub>n'' = virtual_copy \<A>\<^sub>i\<^sub>n';
+    if IsaSAT_use_fast_mode \<and> length CS < uint_max - 1
+    then do {
+        S \<leftarrow> isasat_input_ops.init_state_wl_heur_fast \<A>\<^sub>i\<^sub>n';
+        (T::twl_st_wl_heur_init) \<leftarrow> isasat_input_ops.init_dt_wl_heur_fast \<A>\<^sub>i\<^sub>n'' CS S;
+        let T = convert_state \<A>\<^sub>i\<^sub>n'' T;
+        if \<not>get_conflict_wl_is_None_heur_init T
+        then RETURN (empty_init_code)
+        else if CS = [] then RETURN (empty_conflict_code)
+        else do {
+           ASSERT(\<A>\<^sub>i\<^sub>n'' \<noteq> {#});
+           ASSERT(isasat_input_bounded_nempty \<A>\<^sub>i\<^sub>n'');
+           ASSERT((\<lambda>(M', N', D', Q', W', ((ns, m, fst_As, lst_As, next_search), to_remove), \<phi>, clvls). fst_As \<noteq> None \<and>
+             lst_As \<noteq> None) T);
+           T \<leftarrow> finalise_init_code (T::twl_st_wl_heur_init);
+           ASSERT(isasat_fast T);
+           U \<leftarrow> isasat_input_ops.cdcl_twl_stgy_prog_break_wl_D_heur_break \<A>\<^sub>i\<^sub>n'' T;
+           RETURN (if get_conflict_wl_is_None_heur U then extract_model_of_state_stat U
+             else extract_state_stat U)
+         }
+      }
+    else do {
+        S \<leftarrow> isasat_input_ops.init_state_wl_heur \<A>\<^sub>i\<^sub>n';
+        (T::twl_st_wl_heur_init) \<leftarrow> isasat_input_ops.init_dt_wl_heur \<A>\<^sub>i\<^sub>n'' CS S;
+        let T = convert_state \<A>\<^sub>i\<^sub>n'' T;
+        if \<not>get_conflict_wl_is_None_heur_init T
+        then RETURN (empty_init_code)
+        else if CS = [] then RETURN (empty_conflict_code)
+        else do {
+           ASSERT(\<A>\<^sub>i\<^sub>n'' \<noteq> {#});
+           ASSERT(isasat_input_bounded_nempty \<A>\<^sub>i\<^sub>n'');
+           ASSERT((\<lambda>(M', N', D', Q', W', ((ns, m, fst_As, lst_As, next_search), to_remove), \<phi>, clvls). fst_As \<noteq> None \<and>
+             lst_As \<noteq> None) T);
+           T \<leftarrow> finalise_init_code (T::twl_st_wl_heur_init);
+           U \<leftarrow> isasat_input_ops.cdcl_twl_stgy_prog_wl_D_heur \<A>\<^sub>i\<^sub>n'' T;
+           RETURN (if get_conflict_wl_is_None_heur U then extract_model_of_state_stat U
+             else extract_state_stat U)
+         }
+      }
+    }\<close>
+
+lemma in_class_in_literals_are_in_\<L>\<^sub>i\<^sub>n:
+  assumes \<open>C \<in> set CS\<close>
+  shows \<open>isasat_input_ops.literals_are_in_\<L>\<^sub>i\<^sub>n (mset_set (extract_atms_clss CS {})) (mset C)\<close>
+  apply (auto simp: isasat_input_ops.literals_are_in_\<L>\<^sub>i\<^sub>n_def extract_atms_clss_alt_def
+       isasat_input_ops.\<L>\<^sub>a\<^sub>l\<^sub>l_def all_lits_of_m_def)
+  apply (subst insert_absorb[OF assms, symmetric])
+  apply auto
+  apply (subst (asm)insert_absorb[OF assms, symmetric])
+  apply (subst insert_absorb[OF assms, symmetric])
+  apply auto
+  done
+(* 
+lemma IsaSAT_heur_alt_def:
   \<open>IsaSAT_heur CS = do{
     ASSERT(\<forall>C\<in>set CS. \<forall>L\<in>set C. nat_of_lit L \<le> uint_max);
     let \<A>\<^sub>i\<^sub>n' = mset_set (extract_atms_clss CS {});
@@ -174,8 +288,32 @@ definition IsaSAT_heur :: \<open>nat clause_l list \<Rightarrow> (nat literal li
        U \<leftarrow> isasat_input_ops.cdcl_twl_stgy_prog_wl_D_heur \<A>\<^sub>i\<^sub>n'' T;
        RETURN (if get_conflict_wl_is_None_heur U then extract_model_of_state_stat U
          else extract_state_stat U)
-     }
-  }\<close>
+      }  
+    }\<close>
+ (is \<open>?A = ?B\<close>)
+proof -
+  have [simp]: \<open>ASSERT \<Phi> \<bind> (\<lambda>_. P) \<le> ASSERT \<Phi> \<bind> (\<lambda>_. Q) \<longleftrightarrow> (\<Phi> \<longrightarrow> P \<le> Q)\<close> for \<Phi> P Q
+    using Refine_Basic.le_ASSERTI_pres by auto
+
+  have 1: \<open>?A \<le> ?B\<close>
+    unfolding IsaSAT_heur_def Let_def isasat_input_ops.init_state_wl_heur_fast_def
+    apply (refine_vcg lhs_step_If)
+     apply (auto intro!:  Refine_Basic.bind_mono)
+    apply (subst isasat_input_ops.init_dt_wl_heur_fast_init_dt_wl_heur)
+        apply (auto simp: isasat_input_ops.init_state_wl_heur_def map_fun_rel_def
+        RES_RES_RETURN_RES RETURN_def in_class_in_literals_are_in_\<L>\<^sub>i\<^sub>n)
+    done
+
+  have 2: \<open>?B \<le> ?A\<close>
+    unfolding IsaSAT_heur_def Let_def isasat_input_ops.init_state_wl_heur_fast_def
+    apply (refine_vcg lhs_step_If)
+     apply (auto intro!:  Refine_Basic.bind_mono)
+    apply (subst isasat_input_ops.init_dt_wl_heur_fast_init_dt_wl_heur)
+        apply (auto simp: isasat_input_ops.init_state_wl_heur_def map_fun_rel_def
+        RES_RES_RETURN_RES RETURN_def in_class_in_literals_are_in_\<L>\<^sub>i\<^sub>n)
+    done
+  show ?thesis using 1 2 by simp
+qed *)
 
 lemma (in -)id_mset_list_assn_list_mset_assn:
   assumes \<open>CONSTRAINT is_pure R\<close>
@@ -211,7 +349,28 @@ lemma cdcl_twl_stgy_prog_wl_D_code_ref':
         \<open>virtual_copy_assn \<A>\<^sub>i\<^sub>n (fst a)\<close>])
   done
 
+
+lemma cdcl_twl_stgy_prog_wl_D_break_fast_code_ref':
+  \<open>(uncurry (\<lambda>_. cdcl_twl_stgy_prog_wl_D_fast_code), 
+      uncurry isasat_input_ops.cdcl_twl_stgy_prog_break_wl_D_heur_break)
+  \<in> [\<lambda>(N, S). N = \<A>\<^sub>i\<^sub>n \<and> isasat_input_bounded_nempty \<A>\<^sub>i\<^sub>n \<and> isasat_fast S]\<^sub>a
+     (virtual_copy_assn)\<^sup>k *\<^sub>a
+    (isasat_input_ops.isasat_fast_assn \<A>\<^sub>i\<^sub>n)\<^sup>d \<rightarrow> isasat_input_ops.isasat_assn \<A>\<^sub>i\<^sub>n\<close>
+  unfolding hfref_def hn_refine_def
+  apply (subst in_pair_collect_simp)
+  apply (intro allI impI)
+  subgoal for a c
+    using cdcl_twl_stgy_prog_wl_D_fast_code.refine[of \<A>\<^sub>i\<^sub>n,
+      unfolded in_pair_collect_simp hfref_def hn_refine_def PR_CONST_def,
+      rule_format, of \<open>snd c\<close> \<open>snd a\<close>]
+    by (cases a)
+      (sep_auto simp:
+      dest!: frame_rule_left[of \<open>isasat_input_ops.isasat_fast_assn _ _ _\<close> _ _
+       \<open>virtual_copy_assn \<A>\<^sub>i\<^sub>n (fst a)\<close>])
+  done
+
 declare cdcl_twl_stgy_prog_wl_D_code_ref'[to_hnr, OF refl, sepref_fr_rules]
+declare cdcl_twl_stgy_prog_wl_D_break_fast_code_ref'[to_hnr, OF refl, sepref_fr_rules]
 
 definition get_trail_wl_code :: \<open>twl_st_wll_trail \<Rightarrow> uint32 list option \<times> stats\<close> where
   \<open>get_trail_wl_code = (\<lambda>((M, _), _, _, _, _ ,_ ,_ ,_, _, _, _, stat). (Some M, stat))\<close>
@@ -271,13 +430,25 @@ end
 
 declare isasat_input_ops.extract_model_of_state_stat_hnr[sepref_fr_rules]
 declare isasat_input_ops.finalise_init_hnr[unfolded PR_CONST_def, sepref_fr_rules]
+declare isasat_input_ops.finalise_init_fast_hnr[unfolded PR_CONST_def, sepref_fr_rules]
 sepref_register to_init_state from_init_state get_conflict_wl_is_None_init extract_stats
   isasat_input_ops.init_dt_wl_heur
 declare init_state_wl_heur_hnr[to_hnr, OF refl, sepref_fr_rules]
   init_dt_wl_code.refine[sepref_fr_rules]
  isasat_input_ops.get_stats_code[sepref_fr_rules]
+ init_state_wl_heur_fast_hnr[to_hnr, OF refl, sepref_fr_rules]
+thm init_state_wl_heur_hnr[to_hnr, OF refl, sepref_fr_rules]
 
-(* TODO: make the intermediate level a proper level *)
+lemma uint_max_nat_assn_hnr[sepref_fr_rules]:
+  \<open>(uncurry0 (return uint_max), uncurry0 (RETURN uint_max)) \<in> unit_assn\<^sup>k \<rightarrow>\<^sub>a nat_assn\<close>
+  by sepref_to_hoare sep_auto
+
+text \<open>Crucial and subtil point for the refinement\<close>
+declare convert_state_hnr[to_hnr, OF _ refl, sepref_fr_rules]
+   convert_state_fast_hnr[to_hnr, OF _ refl, sepref_fr_rules]
+sepref_register isasat_input_ops.init_dt_wl_heur_fast
+declare init_dt_wl_fast_code.refine[sepref_fr_rules]
+
 sepref_definition IsaSAT_code
   is \<open>IsaSAT_heur\<close>
   :: \<open>(list_assn (list_assn unat_lit_assn))\<^sup>k \<rightarrow>\<^sub>a model_stat_assn\<close>
@@ -288,6 +459,7 @@ sepref_definition IsaSAT_code
   supply get_conflict_wl_is_None_heur_init_def[simp]
   isasat_input_bounded.get_conflict_wl_is_None_code_refine[sepref_fr_rules]
   isasat_input_bounded.get_conflict_wl_is_None_init_code_hnr[sepref_fr_rules]
+  isasat_input_bounded.get_conflict_wl_is_None_init_fast_code_hnr[sepref_fr_rules]
   isasat_input_ops.to_init_state_hnr[sepref_fr_rules]
   isasat_input_ops.from_init_state_hnr[sepref_fr_rules]
   isasat_input_bounded.get_conflict_wl_is_None_init_wl_hnr[
@@ -296,61 +468,7 @@ sepref_definition IsaSAT_code
    option.splits[split] virtual_copy_def[simp]
    extract_stats_def[simp del]
   apply (rewrite at \<open>extract_atms_clss _ \<hole>\<close> op_extract_list_empty_def[symmetric])
-  apply sepref_dbg_keep
-      apply sepref_dbg_trans_keep
-              apply sepref_dbg_trans_step_keep
-              apply (rule refl)
-  apply sepref_dbg_trans_step_keep
-  apply sepref_dbg_trans_step_keep
-  apply sepref_dbg_trans_step_keep
-  apply sepref_dbg_trans_step_keep
-  apply sepref_dbg_trans_step_keep
-  apply sepref_dbg_trans_step_keep
-  apply sepref_dbg_trans_step_keep
-  apply sepref_dbg_trans_step_keep
-  apply sepref_dbg_trans_step_keep
-  apply sepref_dbg_trans_step_keep
-  apply sepref_dbg_trans_step_keep
-  apply sepref_dbg_trans_step_keep
-  apply sepref_dbg_trans_step_keep
-  apply sepref_dbg_trans_step_keep
-  apply sepref_dbg_trans_step_keep
-  apply sepref_dbg_trans_step_keep
-  apply sepref_dbg_trans_step_keep
-  apply sepref_dbg_trans_step_keep
-  apply sepref_dbg_trans_step_keep
-  apply sepref_dbg_trans_step_keep
-  apply sepref_dbg_trans_step_keep
-  apply sepref_dbg_trans_step_keep
-  apply sepref_dbg_trans_step_keep
-  apply sepref_dbg_trans_step_keep
-  apply sepref_dbg_trans_step_keep
-  apply sepref_dbg_trans_step_keep
-  apply sepref_dbg_trans_step_keep
-  apply sepref_dbg_trans_step_keep
-  apply sepref_dbg_trans_step_keep
-  apply sepref_dbg_trans_step_keep
-  apply sepref_dbg_trans_step_keep
-  apply sepref_dbg_trans_step_keep
-  apply sepref_dbg_trans_step_keep
-  apply sepref_dbg_trans_step_keep
-  apply sepref_dbg_trans_step_keep
-  apply sepref_dbg_trans_step_keep
-  apply sepref_dbg_trans_step_keep
-  apply sepref_dbg_trans_step_keep
-  apply sepref_dbg_trans_step_keep
-  apply sepref_dbg_trans_step_keep
-  apply sepref_dbg_trans_step_keep
-  apply sepref_dbg_trans_step_keep
-  apply sepref_dbg_trans_step_keep
-  apply sepref_dbg_trans_step_keep
-  apply sepref_dbg_trans_step_keep
-                  apply fast
-  apply sepref_dbg_cons_solve
-  apply sepref_dbg_cons_solve
-  apply sepref_dbg_constraints
-  done
-
+  by sepref
 
 definition nth_u_code' where
   [symmetric, code]: \<open>nth_u_code' = nth_u_code\<close>
@@ -1063,44 +1181,107 @@ proof -
         simp del: literal_of_nat.simps)
 qed
 
+lemma (in isasat_input_ops) twl_st_heur_init_vmtf_next_emptyD:
+  \<open>((x1, x1a, x1b, x1c, x1d, ((x1g, x1h, x1i, x1j, x2h), x2i), x1k, x2k), Ta)
+       \<in> twl_st_heur_init \<Longrightarrow> \<A>\<^sub>i\<^sub>n \<noteq> {#} \<Longrightarrow> x1i \<noteq> None\<close>
+  by (auto simp: isasat_input_ops.twl_st_heur_init_def  isasat_input_ops.vmtf_init_def)
 
-lemma [simp]:
-  \<open>(Tb, from_init_state Ta) \<in> isasat_input_ops.twl_st_heur_init_wl A \<Longrightarrow>
+lemma (in isasat_input_ops) twl_st_heur_init_vmtf_fstD:
+  \<open>((x1, x1a, x1b, x1c, x1d, ((x1g, x1h, x1i, x1j, x2h), x2i), x1k, x2k), Ta)
+       \<in> twl_st_heur_init \<Longrightarrow> \<A>\<^sub>i\<^sub>n \<noteq> {#} \<Longrightarrow> x1j \<noteq> None\<close>
+  by (auto simp: isasat_input_ops.twl_st_heur_init_def  isasat_input_ops.vmtf_init_def)
+
+
+
+lemma get_conflict_wl_is_None_init_get_conflict_wl_is_None_heur_init[simp]:
+  \<open>(Tb, Ta) \<in> isasat_input_ops.twl_st_heur_init A \<Longrightarrow>
      get_conflict_wl_is_None_init (from_init_state Ta) = get_conflict_wl_is_None_heur_init Tb\<close>
-  by (auto simp: isasat_input_ops.twl_st_heur_init_wl_def from_init_state_def
+  by (cases Ta; cases Tb)
+   (auto simp: isasat_input_ops.twl_st_heur_init_wl_def from_init_state_def
       get_conflict_wl_is_None_init_def get_conflict_wl_is_None_heur_init_def
-      get_conflict_wl_is_None_def)
+      isasat_input_ops.twl_st_heur_init_def
+      get_conflict_wl_is_None_def split: option.splits)
+
+lemma (in isasat_input_ops) twl_st_heur_init_wl:
+  \<open>(T, Ta) \<in> twl_st_heur_init \<Longrightarrow> (T, from_init_state Ta) \<in> twl_st_heur_init_wl\<close>
+  by (cases T; cases Ta)
+    (auto simp: twl_st_heur_init_def twl_st_heur_init_wl_def from_init_state_def)
 
 lemma IsaSAT_heur_IsaSAT: \<open>(IsaSAT_heur, IsaSAT) \<in>
      [\<lambda>CS.  Multiset.Ball (mset CS) distinct \<and> (\<forall>C\<in>set CS. \<forall>L\<in>set C. nat_of_lit L \<le> uint_max)]\<^sub>f
      Id \<rightarrow> \<langle>{((M, stat), M'). M = M'}\<rangle>nres_rel\<close>
 proof -
   define f :: \<open>twl_st_wl_heur_init \<Rightarrow> twl_st_wl_heur_init nres\<close> where \<open>f = RETURN\<close>
-  have IsaSAT_heur_alt_def:
-    \<open>IsaSAT_heur CS = do{
-     ASSERT (\<forall>C\<in>set CS. \<forall>L\<in>set C. nat_of_lit L \<le> uint_max);
-    let \<A>\<^sub>i\<^sub>n' = mset_set (extract_atms_clss CS {});
-    ASSERT(isasat_input_bounded \<A>\<^sub>i\<^sub>n');
-    ASSERT(distinct_mset \<A>\<^sub>i\<^sub>n');
-    S \<leftarrow> isasat_input_ops.init_state_wl_heur \<A>\<^sub>i\<^sub>n';
-    S \<leftarrow> f S;
-    (T::twl_st_wl_heur_init) \<leftarrow> isasat_input_ops.init_dt_wl_heur \<A>\<^sub>i\<^sub>n' CS S;
-    T \<leftarrow> f T;
-    if \<not>get_conflict_wl_is_None_heur_init T
-    then RETURN (empty_init_code)
-    else if CS = [] then RETURN (empty_conflict_code)
+  have  IsaSAT_heur_alt_def: \<open>IsaSAT_heur CS = do{
+    ASSERT(\<forall>C\<in>set CS. \<forall>L\<in>set C. nat_of_lit L \<le> uint_max);
+    let \<A>\<^sub>i\<^sub>n'' = mset_set (extract_atms_clss CS {});
+    ASSERT(isasat_input_bounded \<A>\<^sub>i\<^sub>n'');
+    ASSERT(distinct_mset \<A>\<^sub>i\<^sub>n'');
+    let b = IsaSAT_use_fast_mode;
+    if b \<and> length CS < uint_max - 1
+    then do {
+        S \<leftarrow> isasat_input_ops.init_state_wl_heur \<A>\<^sub>i\<^sub>n'';
+        S \<leftarrow> f S;
+        (T::twl_st_wl_heur_init) \<leftarrow> isasat_input_ops.init_dt_wl_heur \<A>\<^sub>i\<^sub>n'' CS S;
+        if \<not>get_conflict_wl_is_None_heur_init T
+        then RETURN (empty_init_code)
+        else if CS = [] then RETURN (empty_conflict_code)
+        else do {
+           ASSERT(\<A>\<^sub>i\<^sub>n'' \<noteq> {#});
+           ASSERT(isasat_input_bounded_nempty \<A>\<^sub>i\<^sub>n'');
+           ASSERT((\<lambda>(M', N', D', Q', W', ((ns, m, fst_As, lst_As, next_search), to_remove), \<phi>, clvls). fst_As \<noteq> None \<and>
+             lst_As \<noteq> None) T);
+           T \<leftarrow> finalise_init_code (T::twl_st_wl_heur_init);
+           ASSERT(isasat_fast T);
+           U \<leftarrow> isasat_input_ops.cdcl_twl_stgy_prog_break_wl_D_heur_break \<A>\<^sub>i\<^sub>n'' T;
+           RETURN (if get_conflict_wl_is_None_heur U then extract_model_of_state_stat U
+             else extract_state_stat U)
+         }
+      }
     else do {
-       ASSERT(\<A>\<^sub>i\<^sub>n' \<noteq> {#});
-       ASSERT(isasat_input_bounded_nempty \<A>\<^sub>i\<^sub>n');
-       ASSERT((\<lambda>(M', N', D', Q', W', ((ns, m, fst_As, lst_As, next_search), to_remove), \<phi>, clvls). fst_As \<noteq> None \<and>
-         lst_As \<noteq> None) T);
-       T \<leftarrow> finalise_init_code (T::twl_st_wl_heur_init);
-       U \<leftarrow> isasat_input_ops.cdcl_twl_stgy_prog_wl_D_heur \<A>\<^sub>i\<^sub>n' T;
-       RETURN (if get_conflict_wl_is_None_heur U then extract_model_of_state_stat U
-         else extract_state_stat U)
-     }
-  }\<close> for CS
-    unfolding IsaSAT_heur_def f_def convert_state_def by auto
+        S \<leftarrow> isasat_input_ops.init_state_wl_heur \<A>\<^sub>i\<^sub>n'';
+        S \<leftarrow> f S;
+        (T::twl_st_wl_heur_init) \<leftarrow> isasat_input_ops.init_dt_wl_heur \<A>\<^sub>i\<^sub>n'' CS S;
+        if \<not>get_conflict_wl_is_None_heur_init T
+        then RETURN (empty_init_code)
+        else if CS = [] then RETURN (empty_conflict_code)
+        else do {
+           ASSERT(\<A>\<^sub>i\<^sub>n'' \<noteq> {#});
+           ASSERT(isasat_input_bounded_nempty \<A>\<^sub>i\<^sub>n'');
+           ASSERT((\<lambda>(M', N', D', Q', W', ((ns, m, fst_As, lst_As, next_search), to_remove), \<phi>, clvls). fst_As \<noteq> None \<and>
+             lst_As \<noteq> None) T);
+           T \<leftarrow> finalise_init_code (T::twl_st_wl_heur_init);
+           U \<leftarrow> isasat_input_ops.cdcl_twl_stgy_prog_wl_D_heur \<A>\<^sub>i\<^sub>n'' T;
+           RETURN (if get_conflict_wl_is_None_heur U then extract_model_of_state_stat U
+             else extract_state_stat U)
+         }
+      }
+    }\<close>  (is \<open>?A = ?B\<close>) for CS
+  proof -
+    have [simp]: \<open>ASSERT \<Phi> \<bind> (\<lambda>_. P) \<le> ASSERT \<Phi> \<bind> (\<lambda>_. Q) \<longleftrightarrow> (\<Phi> \<longrightarrow> P \<le> Q)\<close> for \<Phi> P Q
+      using Refine_Basic.le_ASSERTI_pres by auto
+
+    have 1: \<open>?A \<le> ?B\<close>
+      unfolding IsaSAT_heur_def Let_def isasat_input_ops.init_state_wl_heur_fast_def f_def
+        empty_conflict_code_def empty_conflict_code_def empty_init_code_def convert_state_def
+      apply (refine_vcg lhs_step_If)
+       apply (auto intro!:  Refine_Basic.bind_mono)
+      apply (subst isasat_input_ops.init_dt_wl_heur_fast_init_dt_wl_heur)
+      apply (auto simp: isasat_input_ops.init_state_wl_heur_def map_fun_rel_def
+          RES_RES_RETURN_RES RETURN_def in_class_in_literals_are_in_\<L>\<^sub>i\<^sub>n)
+      done
+
+    have 2: \<open>?B \<le> ?A\<close>
+      unfolding IsaSAT_heur_def Let_def isasat_input_ops.init_state_wl_heur_fast_def f_def
+        empty_conflict_code_def empty_conflict_code_def empty_init_code_def convert_state_def
+      apply (refine_vcg lhs_step_If)
+      apply (auto intro!:  Refine_Basic.bind_mono)
+      apply (subst isasat_input_ops.init_dt_wl_heur_fast_init_dt_wl_heur)
+      apply (auto simp: isasat_input_ops.init_state_wl_heur_def map_fun_rel_def
+          RES_RES_RETURN_RES RETURN_def in_class_in_literals_are_in_\<L>\<^sub>i\<^sub>n)
+      done
+    show ?thesis using 1 2 by simp
+  qed
 
   have [refine]: \<open>(T, T') \<in> isasat_input_ops.twl_st_heur_init_wl N \<Longrightarrow>
     f T \<le> \<Down> {(T, (T', OS)). (T, T') \<in> isasat_input_ops.twl_st_heur_init_wl N}
@@ -1179,32 +1360,44 @@ proof -
     subgoal by auto
     subgoal by auto
     subgoal by auto
+    subgoal by auto
+    subgoal by auto
                 apply (assumption)+
     subgoal by auto
-    apply assumption
-                   apply (assumption)+
+    apply (assumption)+
+    subgoal by auto
+    subgoal by (auto simp: empty_init_code_def)
     subgoal for CS CS' S S'
       by simp
-    subgoal
-        by (auto simp: empty_init_code_def)
-      subgoal for CS CS' S S' T T'
-      by (auto simp:  isasat_input_ops.twl_st_heur_init_wl_def
-          get_conflict_wl_is_None_heur_init_def get_conflict_wl_is_None_init_def
-          get_conflict_wl_is_None_def)
     subgoal premises p
       by (auto simp: empty_conflict_code_def)
     subgoal by auto
     subgoal by auto
     subgoal
-      by (auto simp: isasat_input_ops.vmtf_init_def
-          isasat_input_ops.twl_st_heur_init_wl_def)
+      by (auto dest: isasat_input_ops.twl_st_heur_init_vmtf_next_emptyD)
     subgoal
-      by (auto simp: isasat_input_ops.vmtf_init_def
-          isasat_input_ops.twl_st_heur_init_wl_def)
+      by (auto dest!: isasat_input_ops.twl_st_heur_init_vmtf_fstD)
+    subgoal
+      by (auto simp: get_conflict_wl_is_None_init_def get_conflict_wl_is_None_def
+          split: option.splits)
+    apply assumption+
+    subgoal
+      by (rule isasat_input_ops.twl_st_heur_init_wl)
+    subgoal
+      sorry
+    subgoal
+      sorry
+    subgoal premises p
+      using p(26) \<comment> \<open>only last assumption\<close>
+      by (auto simp: extract_model_of_state_stat_def extract_model_of_state_def
+          isasat_input_ops.twl_st_heur_def get_conflict_wl_is_None_heur_def
+          get_conflict_wl_is_None_heur_init_def extract_state_stat_def
+          get_conflict_wl_is_None_def split: option.splits)
     subgoal
       by (auto simp:  isasat_input_ops.twl_st_heur_init_wl_def
           get_conflict_wl_is_None_heur_init_def get_conflict_wl_is_None_init_def
           get_conflict_wl_is_None_def split: option.splits)
+    oops
     apply assumption+
     subgoal ..
     subgoal by simp
